VCVio/OracleComp/OracleSpec.lean
@@ -23,17 +23,27 @@ We also define a number of basic oracle constructions:
 
 universe u u' v w
 
-/-- Oracles are specified by a polynomial functor, where `A` is the index/input of the oracle,
-and `B` gives the output type of the oracle for a given index.
-dt: should we actually have this as an alias? Could in theory drop it completely. -/
-abbrev OracleSpec := PFunctor
+/-- Oracles are specified by a polynomial functor, where `domain` is the index/input of the oracle,
+and `range` gives the output type of the oracle for a given index.
+This type is essentially a copy of `PFunctor` used to hide certain abstractions
+in a form that is more familiar to an average user. -/
+structure OracleSpec where
+  domain : Type u
+  range : domain → Type v
+  deriving Inhabited
 
-example : Inhabited OracleSpec := inferInstance --As (Inhabited (PFunctor))
+namespace OracleSpec
 
-abbrev OracleSpec.domain (spec : OracleSpec) : Type _ := spec.A
+variable {spec : OracleSpec}
 
-/-- Type of the range for calls to the oracle corresponding to index `i`. -/
-abbrev OracleSpec.range (spec : OracleSpec) (i : spec.A) := spec.B i
+instance : Coe OracleSpec PFunctor where
+  coe spec := { A := spec.domain, B := spec.range }
+
+@[simp] lemma coe_def (spec : OracleSpec) :
+    (↑spec : PFunctor) = { A := spec.domain, B := spec.range } := rfl
+
+@[reducible, simp] def ofPFunctor (P : PFunctor) : OracleSpec :=
+  { domain := P.A, range := P.B }
 
 /-- An oracle spec has indexing in a type `ι` if the `range` function factors through `ι`.
 dt: not sure if this is really the right approach for e.g. `pregen`. -/
@@ -42,10 +52,33 @@ class HasIndexing (spec : OracleSpec) (ι : Type w) where
   xdi : ι → Type _
   range_idx (t : spec.domain) : spec.range t = xdi (idx t)
 
-abbrev emptySpec := 0
-notation "[]ₒ" => 0
+protected class Fintype (spec : OracleSpec) extends PFunctor.Fintype ↑spec
+protected class Inhabited (spec : OracleSpec) extends PFunctor.Inhabited ↑spec
+protected class DecidableEq (spec : OracleSpec) extends PFunctor.DecidableEq ↑spec
 
-infixl : 25 " →ₒ " => PFunctor.ofConst
+instance [h : spec.Fintype] (t : spec.domain) : Fintype (spec.range t) := h.fintype_B t
+instance [h : spec.Inhabited] (t : spec.domain) : Inhabited (spec.range t) := h.inhabited_B t
+instance [h : spec.DecidableEq] : DecidableEq spec.domain := h.decidableEq_A
+instance [h : spec.DecidableEq] (t : spec.domain) : DecidableEq (spec.range t) := h.decidableEq_B t
+
+instance : Add OracleSpec where add spec spec' := ofPFunctor (spec + spec')
+
+@[simp] lemma domain_add (spec spec' : OracleSpec) :
+    (spec + spec').domain = (spec.domain ⊕ spec'.domain) := rfl
+
+@[simp] lemma range_add_inl (spec spec' : OracleSpec) (t : spec.domain) :
+    (spec + spec').range (.inl t) = spec.range t := rfl
+
+@[simp] lemma range_add_inr (spec spec' : OracleSpec) (t : spec'.domain) :
+    (spec + spec').range (.inr t) = spec'.range t := rfl
+
+end OracleSpec
+
+def emptySpec : OracleSpec := .ofPFunctor 0
+notation "[]ₒ" => emptySpec
+
+def singletonSpec (A B : Type*) : OracleSpec := .ofPFunctor (PFunctor.ofConst A B)
+infixl : 25 " →ₒ " => singletonSpec
 
 /-- Access to a coin flipping oracle. Because of termination rules in Lean this is slightly
 weaker than `unifSpec`, as we have only finitely many coin flips. -/
@@ -58,8 +91,8 @@ def coinSpec : OracleSpec.{0,0} := Unit →ₒ Bool
 /-- Access to oracles for uniformly selecting from `Fin (n + 1)` for arbitrary `n : ℕ`.
 By adding `1` to the index we avoid selection from the empty type `Fin 0 ≃ empty`.-/
 @[inline, reducible] def unifSpec : OracleSpec.{0,0} where
-  A := ℕ
-  B n := Fin (n + 1)
+  domain := ℕ
+  range n := Fin (n + 1)
 
 @[simp] lemma domain_unifSpec : unifSpec.domain = ℕ := rfl
 @[simp] lemma range_unifSpec (t : unifSpec.domain) : unifSpec.range t = Fin (t + 1) := rfl
@@ -71,5 +104,5 @@ instance : unifSpec.Inhabited where inhabited_B n := inferInstanceAs (Inhabited 
 One question is that we may have empty selection
 Select uniformly from a range (not starting from zero).-/
 @[inline, reducible] def probSpec : OracleSpec.{0,0} where
-  A := ℕ × ℕ
-  B r := Fin (r.2 + 1)
+  domain := ℕ × ℕ
+  range r := Fin (r.2 + 1)
